\documentclass[]{elsarticle}\setlength{\marginparwidth}{0.5in}\usepackage{amsmath,amssymb,amsthm,natbib,mathtools,graphicx}\input FJHDef.tex\DeclareMathOperator{\lin}{lin}\DeclareMathOperator{\up}{up}\DeclareMathOperator{\lo}{lo}\DeclareMathOperator{\fix}{non}\DeclareMathOperator{\err}{err}\DeclareMathOperator{\tol}{tol}\newcommand{\fudge}{\mathfrak{C}}\newtheorem{theorem}{Theorem}\newtheorem{prop}[theorem]{Proposition}\newtheorem{lem}{Lemma}\theoremstyle{definition}\newtheorem{algo}{Algorithm}\newtheorem{condit}{Condition}%\newtheorem{assump}{Assumption}\theoremstyle{remark}\newtheorem{rem}{Remark}\journal{Journal of Complexity}\begin{document}\begin{frontmatter}\title{Asymptotic Error Estimation for Trapezoidal Rule}\author{Fred J. Hickernell}\address{Room E1-208, Department of Applied Mathematics, Illinois Institute of Technology,\\ 10 W.\ 32$^{\text{nd}}$ St., Chicago, IL 60616}\begin{abstract}\end{abstract}\begin{keyword}adaptive \sep cones \sep function recovery \sep integration \sep quadrature%% keywords here, in the form: keyword \sep keyword\MSC[2010] 65D05 \sep 65D30 \sep 65G20%% MSC codes here, in the form: \MSC code \sep code%% or \MSC[2008] code \sep code (2000 is the default)\end{keyword}\end{frontmatter}\section{Problem}Consider the integral \begin{equation*}I(f)= \int_0^1 f(x) \, \dif x\end{equation*}that is approximated by the trapezoidal rule \begin{equation*}\hI_n(f)= \frac{1}{n} \left[ \frac{1}{2}f(0) + f(1/n) + f(2/n) + \cdots +  f (1-1/n) + \frac{1}{2} f(1)\right].\end{equation*}The error is often estimated as \begin{equation*}E_n(f) := I(n) - \hI_n(f) \approx \frac{\hI_n(f)-\hI_{n/2}(f)}{3} =: \hE_n(f).\end{equation*}We want to find a bound on $E_n(f)-\hE_n(f)$.\section{Error for One or Two Trapezoids}Looking at a piece of the trapezoidal rule, given $a$ and $h$ we have\begin{align*}\MoveEqLeft{\int_a^{a+h} f(x) \, \dif x - \frac{h}{2}[f(a)+f(a+h)]}\\& = f(x) (x-a-h/2) \Bigr \rvert_a^{a+h} - \int_a^{a+h} f'(x) (x-a-h/2) \, \dif x \\&\qquad \qquad - \frac{h}{2}[f(a)+f(a+h)] \\& = - \int_a^{a+h} f'(x) (x-a-h/2) \, \dif x \\& = f'(x) \frac{(x-a)(a+h-x)}{2} \Bigr \rvert_a^{a+h} - \int_a^{a+h} f''(x) \frac{(x-a)(a+h-x)}{2} \, \dif x \\& = - \int_a^{a+h} f''(x) \frac{(x-a)(a+h-x)}{2} \, \dif x\end{align*}Thus, for the integral over $[a,a+2h]$ using one trapezoid, the error is \begin{multline} \label{onetraperror}\int_a^{a+2h} f(x) \, \dif x - h[f(a)+f(a+2h)] \\= - \int_a^{a+2h} f''(x) \frac{(x-a)(a+2h-x)}{2} \, \dif x,\end{multline}while the error of the same integral using two trapezoids is\begin{subequations} \label{twotraperror}\begin{align} \nonumberE_2(f) &= \int_a^{a+2h} f(x) \, \dif x - \frac{h}2[f(a)+2f(a+h)+f(a+2h)] \\\nonumber& = - \int_a^{a+2h} f''(x) \left\{\left[\frac{(x-a)(a+h-x)}{2}\right] 1_{[a,a+h]}(x) \right . \\\nonumber& \qquad \qquad \left . + \left[\frac{(x-a-h)(a+2h-x)}{2}\right] 1_{[a+h,a+2h]}(x) \right\} \, \dif x \\& = - \int_a^{a+2h} f''(x) \left[\frac{\abs{x-a-h}(h-\abs{x-a-h})}{2}\right] \dif x \\& = \int_a^{a+2h} f''(x) u(x) \, \dif x,\intertext{where}u(x)& = -\left[\frac{\abs{x-a-h}(h-\abs{x-a-h})}{2}\right] = \Theta(h^2).\end{align}\end{subequations}Since $u(x) = \Theta(h^2)$, it follows that $E_2(f)=\Theta(h^3)$, as expected.An expression for \begin{align*}\hE_2(f) &= \frac{1}{3} \left\{ \frac{h}2[f(a)+2f(a+h)+f(a+2h)] - h[f(a)+f(a+2h)]  \right\} \\& = \frac{h}{6} [-f(a)+2f(a+h)-f(a+2h)]\end{align*}may be obtained from \eqref{onetraperror} and \eqref{twotraperror} as follows:\begin{align*}\hE_2(f) &= \int_a^{a+2h} f''(x) v(x) \, \dif x, \\v(x) &= \frac{1}{3} \left\{ \left[\frac{\abs{x-a-h}(h-\abs{x-a-h})}{2}\right]- \frac{(x-a)(a+2h-x)}{2} \right\} \\& = \frac{1}{6} \left\{ \abs{x-a-h}(h-\abs{x-a-h}) - (x-a)(a+2h-x) \right\}\\& = \frac{1}{6} \left\{ \abs{x-a-h}(h-\abs{x-a-h}) - [h^2- \abs{x-a-h}^2] \right\}\\& = \frac{h}{6} \left\{ \abs{x-a-h} - h \right\}= \Theta(h^2).\end{align*}Since $v(x) = \Theta(h^2)$, it follows that $\hE_2(f)=\Theta(h^3)$, as expected.It is hoped that $E_2(f) - \hE_2(f) = o(h^3)$.  The difference between the true and approximate errors is \begin{align*}E_2(f) - \hE_2(f) &= \int_a^{a+2h} f''(x) w(x) \, \dif x, \\w(x) &= u(x) - v(x) \\&= -\left[\frac{\abs{x-a-h}(h-\abs{x-a-h})}{2}\right] -  \frac{h}{6} \left\{ \abs{x-a-h} - h \right\}\\&=\frac{1}{6} \left[3 (x-a-h)^2 - 4 h \abs{x-a-h} + h^2\right] \\&=\frac{1}{6} (3 \abs{x-a-h} - h)( \abs{x-a-h} - h) = \Theta(h^2).\end{align*}Now let \begin{align*}W(x) &= \int_{a}^x w(t) \, \dif t \\&=\frac{1}{6} \int_{a}^x \left[3 (t-a-h)^2 - 4 h \abs{t-a-h} + h^2\right] \, \dif t\\&=\frac{1}{6} \left . \left[(t-a-h)^3 - 2 h \abs{t-a-h}(t-a-h) + h^2 (t-a-h)\right] \right \rvert_a^x \\&=\frac{1}{6}  \left[(x-a-h)^3 - 2 h \abs{x-a-h}(x-a-h) + h^2 (x-a-h)\right] \\&=\frac{1}{6}  (x-a-h)\left[(x-a-h)^2 - 2 h \abs{x-a-h} + h^2\right] \\&=\frac{1}{6}  (x-a-h)(\abs{x-a-h} - h)^2 = \Theta(h^3).\end{align*}Note that $W(a)=W(a+2h)=0$.  Thus,\begin{align*}E_2(f) - \hE_2(f) &= \int_a^{a+2h} f''(x) w(x) \, \dif x, \\&= f''(x) W(x) \Bigr \rvert_a^{a+h} - \int_a^{a+2h} f'''(x) W(x) \, \dif x \\&= - \int_a^{a+2h} f'''(x) W(x) \, \dif x, \\\abs{E_2(f) - \hE_2(f)} &=\abs{\int_a^{a+2h} f'''(x) W(x) \, \dif x} \\&\le \sup_{a \le x \le a+2h} \abs{W(x)} \times \int_a^{a+2h} \abs{f'''(x)} \, \dif x.\end{align*}Noting that $\abs{W(x)}$ attains its maximum where $w(x)$ vanishes, i.e., at $x=a+h \pm h/3$, and that\[\abs{W(a+h \pm h/3)}= \frac{1}{6} \times \frac{h}{3} \times \left(\frac{2h}{3}\right)^2 = \frac{2h^3}{81}\]it follows that \begin{equation*}\abs{E_2(f) - \hE_2(f)} \le \frac{2h^3}{81} \int_a^{a+2h} \abs{f'''(x)} \, \dif x = \Theta(h^4).\end{equation*}If $f^{(4)}$ is integrable, then one may bound the difference of the true and approximate error better as follows.  Let \begin{align*}\tW(x) &= \int_{a}^x W(t) \, \dif t \\&=\frac{1}{6} \int_{a}^x  (x-a-h)(\abs{x-a-h} - h)^2 \, \dif t\\&=\frac{1}{6} \left . \left[\frac{1}{4}(t-a-h)^4 - \frac{2h}3  \abs{t-a-h}^3 + \frac{h^2}2 (t-a-h)^2\right] \right \rvert_a^x \\&=\frac{1}{72} \left[3(t-a-h)^4 - 8h\abs{t-a-h}^3 + 6h^2 (t-a-h)^2 - h^4\right],\end{align*}and note that $\tW(a)=\tW(a+2h)=0$.  Then it follows that\begin{align*}E_2(f) - \hE_2(f) &= - \int_a^{a+2h} f'''(x) W(x) \, \dif x, \\&= -f'''(x) \tW(x) \Bigr \rvert_a^{a+h} + \int_a^{a+2h} f^{(4)}(x) \tW(x) \, \dif x \\&= \int_a^{a+2h} f^{(4)}(x) \tW(x) \, \dif x, \\\abs{E_2(f) - \hE_2(f)} &=\abs{\int_a^{a+2h} f^{(4)}(x) \tW(x) \, \dif x} \\&\le \sup_{a \le x \le a+2h} \abs{\tW(x)} \times \int_a^{a+2h} \abs{f^{(4)}(x)} \, \dif x.\end{align*}Noting that $\abs{\tW(x)}$ attains its maximum where $W(x)$ vanishes, i.e., at $x=a+h$, and that\[\abs{\tW(a+h)}= \frac{h^4}{72},\]it follows that \begin{equation*}\abs{E_2(f) - \hE_2(f)} \le \frac{h^4}{72} \int_a^{a+2h} \abs{f^{(4)}(x)} \, \dif x = \Theta(h^5).\end{equation*}\section{Error for the Whole Integral}Applying the work from the previous section with $h=1/n$, and $a=x_i$ for $i=0, 2, 4 \ldots, n-2$ it follows that\begin{align*}\abs{E_n(f) - \hE_n/2(f)} & \le \frac{2h^3}{81} \sum_{j=0}^{n/2-1} \int_{x_{2j}}^{x_{2j+2}} \abs{f'''(x)} \, \dif x \\& = \frac{2}{81n^3} \int_{0}^{1} \abs{f'''(x)} \, \dif x  = \frac{2}{81n^3} \norm[1]{f'''},  \\\abs{E_n(f) - \hE_n/2(f)} & \le \frac{h^4}{72} \sum_{j=0}^{n/2-1} \int_{x_{2j}}^{x_{2j+2}} \abs{f^{(4)}(x)} \, \dif x\\& = \frac{1}{72 n^4} \int_{0}^{1} \abs{f^{(4)}(x)} \, \dif x  = \frac{1}{72 n^4}\norm[1]{f^{(4)}}.\end{align*}\bibliographystyle{spbasic}\bibliography{FJH22,FJHown22}\end{document}