\documentclass[]{elsarticle}
\setlength{\marginparwidth}{0.5in}
\usepackage{amsmath,amssymb,amsthm,natbib,mathtools,graphicx}
\input FJHDef.tex

\journal{Journal of Complexity}

\begin{document}

\begin{frontmatter}

\title{Proof of Error of $G_n$}
\author{Fred}

\end{frontmatter}

Given the data sites $x_i=(i-1)/(n-1)$, $i=0, \ldots, n$, let the $\cl_\infty$ norm of the $f'$ be approximated by
\[
G_n(f) = (n-1) \sup_{i=1, \ldots, n-1} \abs{f(x_{i+1})-f(x_i)}
\]
For any $x \in [x_{i}, x_{i+1}]$, note that 
\begin{align*}
\MoveEqLeft{\abs{f'(x)} - (n-1) \abs{f(x_{i+1})-f(x_i)}} \\
 & \le \abs{f'(x) - (n-1)[f(x_{i+1})-f(x_i)]} \\
&=\abs{ \int_{x_i}^{x_{i+1}} f''(t) [(n-1)(t-x_i) -  1_{[x,x_{i+1}]}(t)] \, \dif t} \\
& \le \sup_{x_i \le t \le x_{i+1}} \abs{f''(t)} \int_{x_i}^{x_{i+1}} \abs{  (n-1)(t-x_i) -  1_{[x,x_{i+1}]}(t)} \, \dif t \\
&=\sup_{x_i \le t \le x_{i+1}} \abs{f''(t)} \left \{\frac{1}{2(n-1)} - (x-x_i)[1-(n-1)(x-x_i)] \right\} \\
&\le \frac{1}{2(n-1)}\sup_{x_i \le t \le x_{i+1}} \abs{f''(t)}
\end{align*}
Furthermore, this inequality is tight if $f''$ is constant second derivative and $f'$ does not change sign over $[x_{i}, x_{i+1}]$, and $x=x_i$ or $x_{i+1}$.  Applying the above argument for $i=0, \ldots, n-1$ implies that
\[
\norm[\infty]{f'} - G_n(f) \le \frac{\norm[\infty]{f''}}{2(n-1)}
\]
with equality holding when has a constant second derivative and its first derivative does not change sign over $[0,1]$.
\end{document}
